Source/Dafny/RefinementTransformer.cs
@@ -839,6 +839,8 @@ namespace Microsoft.Dafny
             reporter.Error(MessageSource.RefinementTransformer, n.tok, "{0} '{1}' of {2} {3} cannot be changed, compared to the corresponding {2} in the module it refines, from new to non-new", parameterKind, n.Name, thing, name);
           } else if (!TypesAreSyntacticallyEqual(o.Type, n.Type)) {
             reporter.Error(MessageSource.RefinementTransformer, n.tok, "the type of {0} '{1}' is different from the type of the same {0} in the corresponding {2} in the module it refines ('{3}' instead of '{4}')", parameterKind, n.Name, thing, n.Type, o.Type);
+          } else if (n.DefaultValue != null) {
+            reporter.Error(MessageSource.RefinementTransformer, n.tok, "a refining formal parameter ('{0}') in a refinement module is not allowed to give a default-value expression", n.Name);
           }
         }
       }
